Test/Monomorphization/Polymorphic.lean
@@ -4,14 +4,9 @@ set_option auto.prep.redMode "instances"
 set_option trace.auto.tactic true
 set_option trace.auto.mono true
 
-set_option trace.auto.mono.printConstInst true in
-set_option trace.auto.printLemmas true in
-example (as bs cs ds : List β) : (as ++ bs) ++ (cs ++ ds) = as ++ (bs ++ (cd ++ ds)) := by
-  try auto [List.append_assoc]
-  sorry
+example (as bs cs ds : List β) : (as ++ bs) ++ (cs ++ ds) = as ++ (bs ++ (cs ++ ds)) := by
+  auto [List.append_assoc]
 
-set_option trace.auto.mono.printConstInst true in
-example (as bs cs : List α) (f : α → β) :
+def tjs (as bs cs : List α) (f : α → β) :
   ((as ++ bs) ++ cs).map f = as.map f ++ (bs.map f ++ cs.map f) := by
-  try auto [List.append_assoc, List.map_append]
-  sorry
+  auto [List.append_assoc, List.map_append]
